ROOT
@@ -1,2 +1,3 @@
 session SABLE = AutoCorres +
   theories "Proofs/Refine_AC_A"
+           "Proofs/Memory"
